proof/invariant-abstract/AARCH64/ArchAInvsPre.thy
@@ -15,153 +15,35 @@ context Arch begin
 
 global_naming AARCH64
 
-(* FIXME AARCH64
-lemma canonical_not_kernel_is_user:
-  "\<lbrakk> v \<notin> kernel_mappings; canonical_address v \<rbrakk> \<Longrightarrow> v \<in> user_region "
-  by (simp add: kernel_mappings_def not_le canonical_below_pptr_base_user)
-
-lemma no_user_region_kernel_mappings:
-  "\<lbrakk> p \<in> user_region; p \<in> kernel_mappings \<rbrakk> \<Longrightarrow> False"
-  using kernel_mappings_user_region by blast
-
-lemma kernel_mappings_slots_eq:
-  "canonical_address p \<Longrightarrow>
-   ucast (p >> pt_bits_left max_pt_level) \<in> kernel_mapping_slots \<longleftrightarrow> p \<in> kernel_mappings"
-  apply (simp add: kernel_mappings_def kernel_mapping_slots_def ucast_mask_drop canonical_address_range)
-  apply word_bitwise
-  by (auto simp: canonical_bit_def word_bits_def pt_bits_left_def bit_simps level_defs word_size
-                 rev_bl_order_simps)
-*)
-
 lemma ucast_ucast_mask_low: "(ucast (x && mask asid_low_bits) :: asid_low_index) = ucast x"
   by (rule ucast_mask_drop, simp add: asid_low_bits_def)
 
-(* FIXME AARCH64
-lemma valid_global_table_rights:
-  "\<lbrakk> pt_ptr \<in> riscv_global_pts (arch_state s) level;
-     valid_global_tables s; valid_global_arch_objs s \<rbrakk> \<Longrightarrow>
-   \<exists>pt. pts_of s pt_ptr = Some pt \<and> (\<forall>idx. pte_rights_of (pt idx) = vm_kernel_only)"
-  by (frule (1) global_pts_ofD) (clarsimp simp: valid_global_tables_def Let_def) *)
-
-(* FIXME AARCH64
 lemma ptes_of_idx:
-  "\<lbrakk> ptes_of s (pt_slot_offset level pt_ptr p) = Some pte;
+  "\<lbrakk> ptes_of s (pt_type pt) (pt_slot_offset level pt_ptr p) = Some pte;
      pts_of s pt_ptr = Some pt; pspace_aligned s \<rbrakk> \<Longrightarrow>
-   \<exists>idx. pt idx = pte"
+   \<exists>idx. pt_apply pt idx = pte"
   apply (drule_tac pt_ptr=pt_ptr in pspace_aligned_pts_ofD, simp)
-  apply (fastforce simp: pte_of_def)
-  done
-
-lemma valid_global_arch_objs_global_ptD:
-  "valid_global_arch_objs s \<Longrightarrow>
-   riscv_global_pt (arch_state s) \<in> riscv_global_pts (arch_state s) max_pt_level"
-  by (auto simp: valid_global_arch_objs_def Let_def riscv_global_pt_def)
-
-lemma equal_kernel_mappingsD:
-  "\<lbrakk> vspace_for_asid asid s = Some pt_ptr; pts_of s pt_ptr = Some pt;
-     equal_kernel_mappings s \<rbrakk> \<Longrightarrow> has_kernel_mappings pt s"
-  by (simp add: equal_kernel_mappings_def)
-
-lemma has_kernel_mappingsD:
-  "\<lbrakk> has_kernel_mappings pt s; valid_global_arch_objs s; idx \<in> kernel_mapping_slots;
-     pte = pt idx \<rbrakk> \<Longrightarrow>
-   \<exists>pt'. pts_of s (riscv_global_pt (arch_state s)) = Some pt' \<and> pte = pt' idx"
-  unfolding has_kernel_mappings_def
-  by (fastforce simp: pt_at_eq dest: valid_global_arch_objs_pt_at)
-
-lemma pte_rights_of_kernel:
-  "\<lbrakk> p \<in> kernel_mappings; canonical_address p; valid_global_vspace_mappings s;
-     equal_kernel_mappings s; valid_global_tables s; valid_global_arch_objs s; valid_vspace_objs s;
-     valid_asid_table s; valid_uses s; pspace_aligned s;
-     (\<exists>asid. vspace_for_asid asid s = Some pt_ref) \<or> pt_ref = riscv_global_pt (arch_state s);
-     pt_lookup_slot pt_ref p (ptes_of s) = Some (level, slot); ptes_of s slot = Some pte \<rbrakk>
-   \<Longrightarrow> pte_rights_of pte = vm_kernel_only"
-  apply (clarsimp simp: pt_lookup_slot_def pt_lookup_slot_from_level_def)
-  apply (rename_tac pt_ptr)
-  apply (erule disjE; clarsimp)
-   apply (subgoal_tac "is_aligned pt_ref pt_bits")
-    prefer 2
-    apply (drule (2) vspace_for_asid_valid_pt)
-    apply clarsimp
-    apply (erule pspace_aligned_pts_ofD)
-    apply simp
-   apply (cases "level = max_pt_level")
-    apply (drule pt_walk_level)
-    apply (clarsimp simp flip: kernel_mappings_slots_eq)
-    apply (clarsimp simp: ptes_of_def table_index_offset_pt_bits_left)
-    apply (drule (2) equal_kernel_mappingsD)
-    apply (drule (3) has_kernel_mappingsD)
-    apply clarsimp
-    apply (frule valid_global_arch_objs_global_ptD)
-    apply (drule (2) valid_global_table_rights)
-    apply fastforce
-   apply (drule pt_walk_equal_top_slot_Some[where pt_ptr'="riscv_global_pt (arch_state s)", rotated])
-    apply (erule (7) equal_mappings_pt_slot_offset)
-   apply clarsimp
-   apply (frule (1) valid_global_tablesD, simp)
-   apply (fastforce dest!: ptes_of_idx valid_global_table_rights)
-  apply (frule (1) valid_global_tablesD, simp)
-  apply (fastforce dest!: ptes_of_idx valid_global_table_rights)
-  done
-
-lemma some_get_page_info_kmapsD:
-  "\<lbrakk> get_page_info (aobjs_of s) pt_ref p = Some (b, a, attr, r);
-     p \<in> kernel_mappings; canonical_address p; valid_global_vspace_mappings s;
-     equal_kernel_mappings s; valid_global_tables s; valid_global_arch_objs s;
-     valid_vspace_objs s; valid_asid_table s; valid_uses s; pspace_aligned s;
-     (\<exists>asid. vspace_for_asid asid s = Some pt_ref) \<or> pt_ref = riscv_global_pt (arch_state s) \<rbrakk>
-   \<Longrightarrow> (\<exists>sz. pageBitsForSize sz = a) \<and> r = {}"
-  apply (clarsimp simp: get_page_info_def in_omonad)
-  apply (rename_tac level slot pte)
-  apply (frule (12) pte_rights_of_kernel, simp add: vm_kernel_only_def)
-  apply (clarsimp simp: pte_info_def split: pte.splits)
-  apply (drule pt_lookup_slot_max_pt_level)
-  apply (rule_tac x="vmpage_size_of_level level" in exI)
-  apply simp
-  done
+  sorry (* FIXME AARCH64
+  apply (fastforce simp: level_pte_of_def in_omonad)
+  done *)
 
 lemma pte_info_not_InvalidPTE:
   "pte_info level pte = Some (b, a, attr, r) \<Longrightarrow> pte \<noteq> InvalidPTE"
   by (simp add: pte_info_def split: pte.splits)
 
-lemma valid_global_tables_toplevel_pt:
-  "\<lbrakk> pts_of s (riscv_global_pt (arch_state s)) = Some pt; valid_global_tables s \<rbrakk> \<Longrightarrow>
-   \<forall>idx\<in>- kernel_mapping_slots. pt idx = InvalidPTE"
-  by (simp add: valid_global_tables_def Let_def riscv_global_pt_def)
-
-lemma global_pt_not_invalid_kernel:
-  "\<lbrakk> ptes_of s (pt_slot_offset max_pt_level (riscv_global_pt (arch_state s)) p) = Some pte;
-     pte \<noteq> InvalidPTE; canonical_address p; valid_global_tables s;
-     is_aligned (riscv_global_pt (arch_state s)) pt_bits\<rbrakk>
-   \<Longrightarrow> p \<in> kernel_mappings"
-  apply (clarsimp simp: pte_of_def table_index_offset_pt_bits_left)
-  apply (fastforce simp flip: kernel_mappings_slots_eq dest: valid_global_tables_toplevel_pt)
-  done
-
-lemma get_page_info_gpd_kmaps:
-  "\<lbrakk> valid_global_vspace_mappings s; valid_arch_state s;
-     get_page_info (aobjs_of s) (riscv_global_pt (arch_state s)) p = Some (b, a, attr, r) \<rbrakk>
-     \<Longrightarrow> p \<in> kernel_mappings"
-  apply (clarsimp simp: get_page_info_def in_omonad pt_lookup_slot_def pt_lookup_slot_from_level_def)
-  apply (subst (asm) pt_walk.simps)
-  apply (fastforce dest: pte_info_not_InvalidPTE global_pt_not_invalid_kernel
-                   simp: valid_arch_state_def in_omonad)
-  done
-
 lemma get_vspace_of_thread_reachable:
-  "\<lbrakk> get_vspace_of_thread (kheap s) (arch_state s) t \<noteq> riscv_global_pt (arch_state s);
+  "\<lbrakk> get_vspace_of_thread (kheap s) (arch_state s) t \<noteq> global_pt s;
      valid_uses s \<rbrakk>
    \<Longrightarrow> (\<exists>\<rhd> (max_pt_level, get_vspace_of_thread (kheap s) (arch_state s) t)) s"
   by (auto simp: get_vspace_of_thread_def
-          split: option.splits cap.splits kernel_object.splits arch_cap.splits if_split_asm
+          split: option.splits cap.splits kernel_object.splits arch_cap.splits if_split_asm pt_type.splits
           intro: vspace_for_asid_vs_lookup)
- *)
 
 lemma data_at_aligned:
   "\<lbrakk> data_at sz p s; pspace_aligned s\<rbrakk> \<Longrightarrow> is_aligned p (pageBitsForSize sz)"
   unfolding data_at_def by (auto simp: obj_at_def dest: pspace_alignedD)
 
-lemma is_aligned_ptrFromPAddr_n_eq:
+lemma is_aligned_ptrFromPAddr_n_eq:  (* FIXME AARCH64: might need a different precondition *)
   "sz \<le> canonical_bit \<Longrightarrow> is_aligned (ptrFromPAddr x) sz = is_aligned x sz"
   apply (rule iffI)
    apply (simp add: ptrFromPAddr_def pptrBaseOffset_def pptrBase_def paddrBase_def canonical_bit_def)
@@ -225,10 +107,9 @@ named_theorems AInvsPre_asms
 
 lemma get_vspace_of_thread_asid_or_global_pt:
   "(\<exists>asid. vspace_for_asid asid s = Some (get_vspace_of_thread (kheap s) (arch_state s) t))
-    \<or> get_vspace_of_thread (kheap s) (arch_state s) t = riscv_global_pt (arch_state s)"
-  sorry (* FIXME AARCH64
+    \<or> get_vspace_of_thread (kheap s) (arch_state s) t = global_pt s"
   by (auto simp: get_vspace_of_thread_def
-           split: option.split kernel_object.split cap.split arch_cap.split) *)
+           split: option.split kernel_object.split cap.split arch_cap.split pt_type.splits)
 
 lemma ptable_rights_imp_frame[AInvsPre_asms]:
   assumes "valid_state s"
@@ -238,8 +119,8 @@ lemma ptable_rights_imp_frame[AInvsPre_asms]:
   using assms get_vspace_of_thread_asid_or_global_pt[of s t]
   apply (clarsimp simp: ptable_lift_def ptable_rights_def in_user_frame_def in_device_frame_def
                  split: option.splits)
-  apply (case_tac "x \<in> kernel_mappings")
   sorry (* FIXME AARCH64
+  apply (case_tac "x \<in> kernel_mappings")
    apply (frule (2) some_get_page_info_kmapsD;
             fastforce simp: valid_state_def valid_arch_state_def valid_pspace_def)
   apply (frule some_get_page_info_umapsD)
